src/regular/regex.lean
@@ -23,99 +23,78 @@ inductive regex (S : Type)
 | append    : regex → regex → regex
 | star      : regex → regex
 
-inductive regex_accepts_word : regex S → list S → Prop
-| eps           : regex_accepts_word regex.eps []
-| one           : Π {ch : S}, 
-                    regex_accepts_word (regex.one ch) [ch]
-| append        : Π {l1 l2 : list S} {r1 r2 : regex S}, 
-                    regex_accepts_word r1 l1 → regex_accepts_word r2 l2 →
-                    regex_accepts_word (regex.append r1 r2) (l1 ++ l2)
-| union_left    : Π {l : list S} {r1 r2 : regex S}, 
-                    regex_accepts_word r1 l → 
-                    regex_accepts_word (regex.union r1 r2) l
-| union_right   : Π {l1 : list S} {r1 r2 : regex S}, 
-                    regex_accepts_word r2 l1 → 
-                    regex_accepts_word (regex.union r1 r2) l1
-| star_eps      : Π {r : regex S}, 
-                    regex_accepts_word (regex.star r) []
-| star_append   : Π {r : regex S} {l1 l2 : list S},
-                    regex_accepts_word r l1 → regex_accepts_word (regex.star r) l2 →
-                    regex_accepts_word (regex.star r) (l1 ++ l2)
+inductive regex.accepts : regex S → list S → Prop
+| eps : 
+    regex.accepts regex.eps []
+| one {ch : S} : 
+    regex.accepts (regex.one ch) [ch]
+| append {l1 l2 r1 r2} :
+    regex.accepts r1 l1 → 
+    regex.accepts r2 l2 →
+    regex.accepts (regex.append r1 r2) (l1 ++ l2)
+| union_left {l r1 r2} :  
+    regex.accepts r1 l → 
+    regex.accepts (regex.union r1 r2) l
+| union_right {l r1 r2} :
+    regex.accepts r2 l →
+    regex.accepts (regex.union r1 r2) l
+| star_eps {r} :
+    regex.accepts (regex.star r) []
+| star_append {r l1 l2} : 
+    regex.accepts r l1 → 
+    regex.accepts (regex.star r) l2 →
+    regex.accepts (regex.star r) (l1 ++ l2)
 
-open regex_accepts_word
 
-@[simp] def lang_of_regex (r : regex S) : set (list S) := {w : list S | regex_accepts_word r w}
+def regex_lang (l : set (list S)) := ∃ r : regex S, r.accepts = l 
 
-def regex_lang (l : set (list S)) := ∃ {r : regex S}, l = lang_of_regex r
+lemma regex_empty_not_accepts {w : list S} : ¬ regex.empty.accepts w := λ h, by cases h
 
-@[simp] lemma mem_lang_iff_accepts 
-    {L : set (list S)} {r : regex S} {w : list S} 
-    (regR : L = lang_of_regex r) : w ∈ L ↔ regex_accepts_word r w := 
-begin
-    split; finish,
-end
-
-theorem regex_empty_is_empty_lang : lang_of_regex (regex.empty : regex S) = ∅ :=
-begin
-    rw set.eq_empty_iff_forall_not_mem,
-    rintro x ⟨_⟩,
-end
+theorem regex_empty_is_empty_lang : regex.empty.accepts = (∅ : set (list S)) :=
+    by {ext, split; rintro ⟨⟩}
 
 theorem empty_is_regex : regex_lang (∅ : set (list S)) := 
-begin
-    use regex.empty,
-    rw regex_empty_is_empty_lang,
-end
+    ⟨regex.empty, regex_empty_is_empty_lang⟩
 
-theorem regex_eps_is_eps_lang : lang_of_regex (regex.eps : regex S) = { [] } :=
+theorem regex_eps_is_eps_lang : regex.eps.accepts = ({[]} : set (list S)) :=
 begin
     ext x, split, {
         rintro ⟨_⟩,
         simp only [set.mem_singleton], 
     }, {
-        intro xnil, 
-        convert regex_accepts_word.eps,
-        apply_instance,
+        intro xnil,
+        convert regex.accepts.eps,
     }
 end
 
 theorem eps_is_regex : regex_lang ({[]} : set (list S)) := 
-begin
-    use regex.eps,
-    rw regex_eps_is_eps_lang,
-end
+    ⟨regex.eps, regex_eps_is_eps_lang⟩
 
-
-theorem regex_one_is_one_lang {ch : S} : lang_of_regex (regex.one ch) = { [ch] } :=
+theorem regex_one_is_one_lang {ch : S} : (regex.one ch).accepts = ({[ch]} : set (list S)) :=
 begin
     ext x, split, {
         rintro ⟨_⟩,
         simp only [set.mem_singleton], 
     }, {
         intro xone, 
-        convert regex_accepts_word.one,
-        apply_instance,
+        convert regex.accepts.one,
     }
 end
 
 theorem one_is_regex {c : S} : regex_lang ({[c]} : set (list S)) := 
-begin
-    use regex.one c,
-    rw regex_one_is_one_lang,
-end
+    ⟨regex.one c, regex_one_is_one_lang⟩
 
 theorem regex_union_is_lang_union {rl rm : regex S}
-    : lang_of_regex (regex.union rl rm) = lang_of_regex rl ∪ lang_of_regex rm :=
+    : (regex.union rl rm).accepts = (rl.accepts ∪ rm.accepts : set (list S)) :=
 begin
-    apply set.subset.antisymm, {
-        rintro x ⟨_⟩,
-        left, assumption,
-        right, assumption
-    }, {
-        rintro x (hleft | hright),
-        exact regex_accepts_word.union_left hleft, 
-        exact regex_accepts_word.union_right hright,
-    }, 
+    apply set.subset.antisymm, 
+    { rintro x (_ | _),
+      left, assumption,
+      right, assumption },
+    { rintro x (hleft | hright),
+      exact regex.accepts.union_left hleft, 
+      exact regex.accepts.union_right hright,
+    },
 end
 
 theorem union_is_regex {L M : set (list S)}: regex_lang L → regex_lang M → regex_lang (L ∪ M) := 
@@ -125,89 +104,62 @@ begin
     rw regex_union_is_lang_union,
 end
 
-theorem regex_append_is_lang_append {rl rm : regex S}
-    : lang_of_regex (regex.append rl rm) = lang_of_regex rl * lang_of_regex rm :=
+theorem regex_append_is_lang_append {rl rm : regex S} :
+    (rl.append rm).accepts = (rl.accepts * rm.accepts : set (list S)) :=
 begin
     apply set.subset.antisymm, {
-        rintro x hx,
-        rcases hx with _ | _ | ⟨ left, right, _, _, hleft, hright ⟩ | _ | _ | _ | _, -- fun with seven cases
+        rintro x h,
+        rcases h with (_ | _ | ⟨left, right, _, _, hleft, hright⟩ | _ | _ | _ | _),
         use [left, right, hleft, hright, rfl], 
     }, {
         rintro _ ⟨ left, right, hleft, hright, rfl ⟩,
-        exact regex_accepts_word.append hleft hright,
+        exact regex.accepts.append hleft hright,
     }
 end
 
 theorem append_is_regex {L M : set (list S)}: regex_lang L → regex_lang M → regex_lang (L * M) := 
 begin
     rintro ⟨rl, rfl⟩ ⟨rm, rfl⟩,
-    use regex.append rl rm,
-    rw regex_append_is_lang_append,
+    exact ⟨regex.append rl rm, regex_append_is_lang_append⟩,
 end
 
-lemma regex_star_iff_list_join {L : set (list S)} {r rs: regex S} 
-    (hr : L = lang_of_regex rs) (w : list S) (hrs : r = rs.star) :
-    regex_accepts_word r w ↔ ∃ l (h : ∀ x, x ∈ l → x ∈ L), w = list.join l :=
+lemma regex_star_iff_list_join {r rs : regex S} 
+    (hrs : rs = r.star) (w : list S)  :
+    rs.accepts w ↔ ∃ l (h : ∀ x, x ∈ l → r.accepts x), w = list.join l :=
 begin
-    subst hr, 
     split, {
-        intro regex_accepts,
-        induction regex_accepts with _ _ _ _ _ _ _ _ _ _ _ _ _ _ _ _ _ _ _ _ _ left right rleft rright ih_left ih_right,
-        repeat {contradiction}, {
+        intro rsw,
+        induction rsw,
+        repeat {contradiction},
+        case star_eps : {
             use list.nil,
-            split; simp,
-        }, {
-            have hrs2 := regex.star.inj hrs,
-            subst hrs2,
-            clear w ih_left hrs,
-            rcases (ih_right rfl) with ⟨ l, h, rfl ⟩,
-            use left :: l,
-            split, {
-                rintro x (xl | xl),
-                rwa ← xl at rleft,
-                exact h _ xl,
-            }, {
-                simp only [list.join], 
-            }
-        }
+            simp,
+        },
+        case star_append : _ left right rleft rright ih_left ih_right {
+            rcases hrs with ⟨_⟩,
+            rcases ih_right hrs with ⟨l, h, rfl⟩,
+            refine ⟨left :: l, _, rfl⟩,
+            rw list.ball_cons,
+            exact ⟨rleft, h⟩,
+        },
     }, {
         subst hrs,
         rintro ⟨l, h, rfl⟩,
         induction l with head tail ih, {
-            use regex_accepts_word.star_eps, 
+            use regex.accepts.star_eps, 
         }, {
-            apply regex_accepts_word.star_append,
-            apply h,
-            simp only [list.mem_cons_iff, true_or, eq_self_iff_true],
-            apply ih,
-            rintro x hx,
-            apply h,
-            simp only [hx, list.mem_cons_iff, or_true],
+            rw list.ball_cons at h,
+            refine regex.accepts.star_append (h.1) (ih h.2),
         },
     },
 end
 
 theorem regex_star_is_kleene_star {rl : regex S}
-    : lang_of_regex rl.star = kleene_star (lang_of_regex rl) :=
+    : rl.star.accepts = kleene_star (rl.accepts) :=
 begin
-    apply set.subset.antisymm, {
-        rintro x hx,
-        rw [star_eq_list_join],
-        exact (regex_star_iff_list_join rfl x rfl).1 hx,
-    }, {
-        suffices hyp : ∀ n, (lang_of_regex rl)^n ⊆ lang_of_regex rl.star, {
-            rintro x ⟨ n, hx ⟩,
-            exact hyp n hx,
-        },
-        intro n,
-        induction n with n hyp, {
-            simp [regex_accepts_word.star_eps], 
-        }, {
-            rw pow_succ,
-            rintro _ ⟨left, right, hleft, hright, rfl⟩,
-            exact regex_accepts_word.star_append hleft (hyp hright),
-        },
-    }
+    ext w,
+    rw star_eq_list_join,
+    exact regex_star_iff_list_join rfl w,
 end
 
 theorem star_is_regex {L : set (list S)}: regex_lang L → regex_lang (kleene_star L) := 
