src/automata/dfa_equivalence.lean
@@ -1,0 +1,213 @@
+import data.fintype.basic
+
+structure dfa (S : Type) [fintype S] :=
+  (Q : Type) -- states
+  [Qfin : fintype Q]
+  (start : Q) -- starting state
+  (term : set Q) -- terminal states
+  (next : Q → S → Q) -- transitions
+
+variables {S : Type} [fintype S] (d : dfa S)
+
+namespace dfa
+
+open_locale classical
+noncomputable theory
+
+instance : fintype d.Q := d.Qfin
+
+def go {d : dfa S} : d.Q → list S → d.Q
+| q []             := q
+| q (head :: tail) := go (d.next q head) tail
+
+@[simp] lemma go_nil (a : d.Q) : go a [] = a := rfl
+@[simp] lemma go_cons (a : d.Q) (head : S) (tail : list S) : go a (head :: tail) = go (d.next a head) tail := rfl
+
+@[simp] lemma go_append (q : d.Q) (u v : list S) :
+  go q (u ++ v) = go (go q u) v :=
+begin
+  induction u with hd tl ih generalizing q, {
+    simp,
+  }, {
+    specialize ih (d.next q hd),
+    simpa using ih,
+  }
+end
+
+def state_equiv (d : dfa S) (u v : d.Q) := ∀ (w : list S), go u w ∈ d.term ↔ go v w ∈ d.term
+
+@[simp] lemma state_equiv_def (u v : d.Q) : state_equiv d u v = ∀ w, go u w ∈ d.term ↔ go v w ∈ d.term := rfl
+
+lemma state_equiv_reflexive : reflexive (state_equiv d) := λ v, by simp
+
+lemma state_equiv_symmetric : symmetric (state_equiv d) := λ u v h w, by simp only [h w]
+
+lemma state_equiv_transitive : transitive (state_equiv d) := λ a b c hab hbc w, by simp only [hab w, hbc w]
+
+lemma state_equiv_equivalence: equivalence (state_equiv d) :=
+  ⟨state_equiv_reflexive d, state_equiv_symmetric d, state_equiv_transitive d⟩
+
+instance setoid : setoid d.Q := ⟨state_equiv d, state_equiv_equivalence d⟩
+
+def Q' (d : dfa S) := quotient d.setoid
+
+@[simp] lemma state_equiv_equiv (a b : d.Q) : a ≈ b ↔ ∀ w, go a w ∈ d.term ↔ go b w ∈ d.term := by refl
+
+def term' (d : dfa S) : set d.Q' := quotient.lift (d.term)
+begin
+  rintro a b hab,
+  specialize hab [],
+  simpa using hab,
+end
+
+def next' (d : dfa S) (c : S) : d.Q' → d.Q' := quotient.lift (λ q, ⟦d.next q c⟧)
+begin
+  rintro a b hab,
+  dsimp only,
+  rw [quotient.eq, state_equiv_equiv],
+  intro w,
+  specialize hab (c :: w),
+  simpa using hab,
+end
+
+def min_dfa (d : dfa S) : dfa S :=
+  { Q := Q' d,
+    Qfin := quotient.fintype _,
+    start := ⟦d.start⟧,
+    term  := term' d,
+    next  := λ q c, next' d c q}
+
+@[simp] lemma min_dfa_Q {d : dfa S} : (min_dfa d).Q = quotient (d.setoid) := rfl
+@[simp] lemma min_dfa_start {d : dfa S} : (min_dfa d).start = ⟦d.start⟧ := rfl
+@[simp] lemma min_dfa_term {d : dfa S} {q} : ⟦q⟧ ∈ (min_dfa d).term ↔ q ∈ d.term := by refl
+@[simp] lemma min_dfa_next {d : dfa S} {q} {c : S}: (min_dfa d).next ⟦q⟧ c = ⟦d.next q c⟧ := by refl
+@[simp] theorem min_dfa_go (d : dfa S) {a} {w}: @go _ _ (min_dfa d) ⟦a⟧ w = ⟦go a w⟧ :=
+begin
+  induction w with head tail ih generalizing a, {
+    simp only [state_equiv_equiv, forall_const, state_equiv_def, iff_self, go_nil],
+  }, {
+    specialize @ih (d.next a head),
+    rw [go, go],
+    exact ih,
+  },
+end
+
+def language (d : dfa S) := {w | go d.start w ∈ d.term}
+
+@[simp] lemma mem_dfa_language_iff {w : list S} {d : dfa S} : 
+  w ∈ d.language ↔ go d.start w ∈ d.term := iff.rfl
+
+theorem min_dfa_lang_eq_dfa_lang (d : dfa S) : d.language = (min_dfa d).language :=
+begin
+  ext,
+  simp,
+end
+
+theorem min_dfa_card_le (d : dfa S) : fintype.card (min_dfa d).Q ≤ fintype.card d.Q := 
+begin
+  simp,
+  exact fintype.card_quotient_le (dfa.setoid d),
+end
+
+def all_reachable (d : dfa S) := ∀ q : d.Q, ∃ w, go d.start w = q
+
+lemma min_dfa_all_reachable {d : dfa S} : d.all_reachable → (min_dfa d).all_reachable :=
+begin
+  rintro hd q,
+  apply quotient.induction_on q, clear q,
+  intro q,
+  rcases hd q with ⟨w, rfl⟩,
+  use w,
+  simp,
+end
+
+end dfa
+
+namespace right_ctx 
+
+variable {L : set (list S)}
+
+def r (L : set (list S)) (u v : list S) := ∀ w, (u ++ w) ∈ L ↔ (v ++ w) ∈ L
+
+@[simp] lemma r_def {u v} : (r L) u v ↔ ∀ w, (u ++ w) ∈ L ↔ (v ++ w) ∈ L := iff.rfl
+
+def r_refl : reflexive (r L) :=
+begin
+  intro u,
+  simp,
+end 
+
+def r_symm : symmetric (r L) := 
+begin
+  intros u v h w,
+  simp [h w],
+end
+
+def r_trans : transitive (r L) :=
+begin
+  intros u v w huv hwv x,
+  simp [huv x, hwv x],
+end
+
+instance setoid : setoid (list S) := ⟨r L, r_refl, r_symm, r_trans⟩
+
+instance has_equiv : has_equiv (list S) := ⟨r L⟩
+
+#check @right_ctx.setoid
+
+def right_ctx (L : set (list S)) := quotient (@right_ctx.setoid S _ L)
+
+#reduce (setoid.r : list S → list S → Prop)
+#reduce (has_equiv.equiv : list S → list S → Prop)
+
+-- @[simp] lemma right_ctx_equiv (u v : list S) :
+--   u ≈ v ↔ ∀ w, (u ++ w) ∈ L ↔ (v ++ w) ∈ L := iff.rfl
+
+end right_ctx
+
+namespace myhill_nerode
+
+open dfa right_ctx
+
+def myhill_nerode_equiv {d : dfa S} (hd : d.all_reachable): (min_dfa d).Q ≃ (right_ctx d.language) :=
+begin
+  letI := @right_ctx.setoid S _ d.language, 
+  exact { 
+    to_fun := quotient.map (λ q, classical.some (hd q))
+    begin
+      rintro a b rab,
+      simp at rab,
+      simp [has_equiv.equiv, setoid.r, r],
+      intro w,
+      specialize rab w,
+      have ha := classical.some_spec (hd a),
+      have hb := classical.some_spec (hd b),
+      rw [ha, hb],
+      exact rab,
+    end,
+    inv_fun := quotient.lift (λ w, go (min_dfa d).start w)
+    begin
+      rintro u v ruv,
+      simp at ⊢ ruv,
+      simpa [has_equiv.equiv, setoid.r] using ruv,
+    end,
+    left_inv := λ q,  
+    begin
+      apply quotient.induction_on q, clear q, intro q,
+      simp,
+      intro w,
+      have hq := classical.some_spec (hd q),
+      rw hq,      
+    end,
+    right_inv := λ w,
+    begin
+      apply quotient.induction_on w, clear w, intro w,
+      simp [has_equiv.equiv, setoid.r],
+      intro x,
+      have hw := classical.some_spec (hd (go d.start w)),
+      rw hw,
+    end
+  },
+end
+
+end myhill_nerode
