src/regular/nonregular.lean
@@ -4,31 +4,30 @@ import regular.regex
 import regular.list_lemmas
 import regular.pumping_lemma 
 
-open dfa list pumping
+open DFA list pumping
 
 def L0ⁿ1ⁿ := {w | ∃ n, w = (repeat bool.ff n) ++ (repeat bool.tt n)}
 
 @[simp] lemma mem_L0ⁿ1ⁿ_iff {w} : w ∈ L0ⁿ1ⁿ ↔ ∃ n, w = (repeat bool.ff n) ++ (repeat bool.tt n) := 
-  by simp only [L0ⁿ1ⁿ, set.mem_set_of_eq]
+  iff.rfl
 
 theorem not_regular_0ⁿ1ⁿ : ¬dfa_lang L0ⁿ1ⁿ :=
 begin
     apply pumping_lemma_negation,
     intro n,
     use [(repeat bool.ff n) ++ (repeat bool.tt n), n],
-    rw length_append,
-    simp only [not_exists, true_and, length_repeat, zero_le, le_add_iff_nonneg_left,
-  set.mem_set_of_eq],
+    simp only [not_exists, true_and, length_repeat, zero_le, le_add_iff_nonneg_left, mem_L0ⁿ1ⁿ_iff,
+  length_append],
     rintro x y z hxyz ynil hpref,
     use 0,
-    simp only [L0ⁿ1ⁿ, not_exists, join, repeat, set.mem_set_of_eq, append_nil],
+    simp only [join, repeat, append_nil],
     rintro l hl,
-    rw ← length_repeat ff n at hpref,
+    rw [← length_repeat ff n, ← length_append] at hpref,
     have tt_n_suffix := suffix_of_append_eq_append hpref hxyz,
-    have tt_eq_ff := repeat_suffix_of_append_repeat _ (suffix_trans tt_n_suffix ⟨x, hl⟩),
+    have tt_eq_ff := repeat_suffix_of_append_repeat _ (is_suffix.trans tt_n_suffix ⟨x, hl⟩),
     contradiction,
     apply_fun length at hxyz hl,
-    simp only [length_repeat, append_assoc, length_append] at hxyz hl,
+    simp only [length_repeat, length_append] at hpref hl hxyz,
     rw [← length_pos_iff_ne_nil] at ynil,
     linarith,
 end
